Specify `Context.Done()` by adding `PCancel` to the logical
description of a `Context`; simplify closeable chan spec

new/proof/chan_proof/closeable.v
@@ -19,30 +19,34 @@ Section proof.
 Context `{hG: heapGS Σ, !ffi_semantics _ _}.
 Context `{closeable_chanG Σ}.
 
-Local Definition own_closeable_chan γch : iProp Σ :=
-  ghost_var γch.(tok_gn) 1 ().
-
 (* Note: could make the namespace be user-chosen *)
-Definition is_closeable_chan V `{!IntoVal V} (ch : chan.t) γch (Pclose : iProp Σ) : iProp Σ :=
-  "#His_ch" ∷ is_chan V ch ∗
+Local Definition is_closeable_chan_internal (ch : chan.t) γch (Pclose : iProp Σ) : iProp Σ :=
+  "#His_ch" ∷ is_chan unit ch ∗
   "#Hinv" ∷ inv nroot (
-      ∃ (st : chanstate.t V),
+      ∃ (st : chanstate.t unit),
         "ch" ∷ own_chan ch st ∗
         "%Hempty" ∷ ⌜ length st.(chanstate.sent) = γch.(init_len) ⌝ ∗
         "%Hle" ∷ ⌜ length st.(chanstate.sent) ≤ st.(chanstate.received) ⌝ ∗
         "#HPclosed" ∷ (if st.(chanstate.closed) then (□ Pclose) else True) ∗
-        "Hclosed" ∷ (if st.(chanstate.closed) then own_closeable_chan γch else True)
+        "Hclosed" ∷ (if st.(chanstate.closed) then ghost_var γch.(tok_gn) 1 () else True)
     ).
+
+Definition own_closeable_chan ch Pclose : iProp Σ :=
+  ∃ γch, is_closeable_chan_internal ch γch Pclose ∗ ghost_var γch.(tok_gn) 1 ().
+#[global] Opaque own_closeable_chan.
+#[local] Transparent own_closeable_chan.
+
+(* Note: could make the namespace be user-chosen *)
+Definition is_closeable_chan (ch : chan.t) (Pclose : iProp Σ) : iProp Σ :=
+  ∃ γch, is_closeable_chan_internal ch γch Pclose.
 #[global] Opaque is_closeable_chan.
 #[local] Transparent is_closeable_chan.
-#[global] Instance is_closeable_chan_pers V `{!IntoVal V} γch ch P :
-  Persistent (is_closeable_chan V γch ch P) := _.
+#[global] Instance is_closeable_chan_pers ch P :
+  Persistent (is_closeable_chan ch P) := _.
 
-Context `{!IntoVal V}.
-Context `{!IntoValTyped V t}.
-Lemma closeable_chan_receive ch γch Pclosed Φ :
-  is_closeable_chan V ch γch Pclosed -∗
-  (Pclosed -∗ Φ (#(default_val V), #false)%V) -∗ receive_atomic_update ch Φ (V:=V).
+Lemma closeable_chan_receive ch Pclosed Φ :
+  is_closeable_chan ch Pclosed -∗
+  (Pclosed -∗ Φ (#(), #false)%V) -∗ receive_atomic_update ch Φ (V:=unit).
 Proof.
   iNamed 1. iIntros "HΦ". rewrite /receive_atomic_update.
   iInv "Hinv" as "Hi" "Hclose". iApply fupd_mask_intro; [ solve_ndisj | iIntros "Hmask"].
@@ -61,12 +65,12 @@ Proof.
     exfalso. apply lookup_lt_Some in Hbad. lia.
 Qed.
 
-Lemma wp_closeable_chan_close ch γch Pclosed Φ :
-  is_closeable_chan V ch γch Pclosed ∗ own_closeable_chan γch ∗ □ Pclosed -∗
+Lemma wp_closeable_chan_close ch Pclosed Φ :
+  own_closeable_chan ch Pclosed ∗ □ Pclosed -∗
   Φ #() -∗
   WP chan.close #ch {{ Φ }}.
 Proof.
-  iIntros "(#His & Hown & #HP) HΦ". iNamed "His".
+  iIntros "(Hown & #HP) HΦ". iDestruct "Hown" as (?) "(His & Hown)". iNamed "His".
   unshelve wp_apply (wp_chan_close with "[$]"); try tc_solve.
   iInv "Hinv" as "Hi" "Hclose". iApply fupd_mask_intro; [ solve_ndisj | iIntros "Hmask"].
   iNext. iNamed "Hi". iFrame. destruct (st.(chanstate.closed)).
@@ -76,18 +80,17 @@ Proof.
   iFrame "∗#%".
 Qed.
 
-Lemma alloc_closeable_chan {E} Pclose ch (s : chanstate.t V) :
+Lemma alloc_closeable_chan {E} Pclose ch (s : chanstate.t unit) :
   s.(chanstate.received) = length s.(chanstate.sent) →
   s.(chanstate.closed) = false →
-  is_chan V ch -∗
   own_chan ch s ={E}=∗
-  ∃ γch,
-  is_closeable_chan V ch γch Pclose ∗
-  own_closeable_chan γch.
+  is_closeable_chan ch Pclose ∗
+  own_closeable_chan ch Pclose.
 Proof.
-  intros ? Hnotclosed. iIntros "His Hch".
+  intros ? Hnotclosed. iIntros "Hch". iDestruct (own_chan_is_chan with "[$]") as "#His".
   iMod (ghost_var_alloc ()) as (tok_gn) "Htok".
-  iExists _. instantiate (1:=ltac:(econstructor)).
+  iAssert (|={E}=> is_closeable_chan_internal ch ltac:(econstructor) Pclose)%I with "[-Htok]" as ">#H".
+  2:{ iFrame "∗#". simpl. iFrame. done. }
   simpl. iFrame.
   iMod (inv_alloc with "[-]") as "$"; last done.
   iFrame. rewrite Hnotclosed. simpl.
